@@ -369,3 +369,4 @@ import Xv6.SpecVirtioDiskRw
 import Xv6.SpecVirtioDiskIntr
 import Xv6.DiskAcc
 import Xv6.PlicPlan
+import Xv6.PlicInv
